src/CSL/Adequacy.v
@@ -1,0 +1,276 @@
+Require Import Spec.Proc.
+Require Import Spec.ProcTheorems.
+Require Import Spec.Abstraction.
+Require Import Spec.Layer.
+Require Import Helpers.RelationAlgebra.
+Require Import Helpers.RelationTheorems.
+Require Import Helpers.RelationRewriting.
+Require Import CSL.WeakestPre.
+Require Import CSL.Crash.
+
+
+
+From stdpp Require Import namespaces.
+From iris.algebra Require Import gmap auth agree gset coPset.
+From iris.base_logic.lib Require Import wsat.
+From iris.proofmode Require Import tactics.
+Set Default Proof Using "Type".
+Import uPred.
+
+(* Global functor setup *)
+Definition invΣ : gFunctors :=
+  #[GFunctor (authRF (gmapURF positive (agreeRF (laterCF idCF))));
+    GFunctor coPset_disjUR;
+    GFunctor (gset_disjUR positive)].
+
+Class invPreG (Σ : gFunctors) : Set := WsatPreG {
+  inv_inPreG :> inG Σ (authR (gmapUR positive (agreeR (laterC (iPreProp Σ)))));
+  enabled_inPreG :> inG Σ coPset_disjR;
+  disabled_inPreG :> inG Σ (gset_disjR positive);
+}.
+
+Instance subG_invΣ {Σ} : subG invΣ Σ → invPreG Σ.
+Proof. solve_inG. Qed.
+
+(* Allocation *)
+Lemma wsat_alloc `{invPreG Σ} : (|==> ∃ _ : invG Σ, wsat ∗ ownE ⊤)%I.
+Proof.
+  iIntros.
+  iMod (own_alloc (● (∅ : gmap _ _))) as (γI) "HI"; first done.
+  iMod (own_alloc (CoPset ⊤)) as (γE) "HE"; first done.
+  iMod (own_alloc (GSet ∅)) as (γD) "HD"; first done.
+  iModIntro; iExists (WsatG _ _ _ _ γI γE γD).
+  rewrite /wsat /ownE -lock; iFrame.
+  iExists ∅. rewrite fmap_empty big_opM_empty. by iFrame.
+Qed.
+
+(* Program logic adequacy *)
+Record adequate {OpT T} {Λ: Layer OpT} (s : stuckness) (e1 : proc OpT T) (σ1 : Λ.(State))
+    (φ : T → Λ.(State) → Prop) := {
+  adequate_result σ2 res :
+    Λ.(exec) e1 σ1 σ2 res → ∃ v, res = existT _ v ∧ φ v σ2;
+  adequate_not_stuck t2 σ2 e2 :
+   s = NotStuck →
+   Λ.(exec_partial) e1 σ1 σ2 t2 →
+   e2 ∈ t2 → (is_Some (to_val (projT2 e2)) ∨ reducible (projT2 e2) σ2)
+}.
+
+(*
+Theorem adequate_tp_safe {OpT T} {Λ: Layer OpT} (e1 : proc OpT T) t2 σ1 σ2 φ :
+  adequate NotStuck e1 σ1 φ →
+  Λ.(step ([e1], σ1) (t2, σ2) →
+  Forall (λ e, is_Some (to_val e)) t2 ∨ ∃ t3 σ3, step (t2, σ2) (t3, σ3).
+Proof.
+  intros Had ?.
+  destruct (decide (Forall (λ e, is_Some (to_val e)) t2)) as [|Ht2]; [by left|].
+  apply (not_Forall_Exists _), Exists_exists in Ht2; destruct Ht2 as (e2&?&He2).
+  destruct (adequate_not_stuck NotStuck e1 σ1 φ Had t2 σ2 e2) as [?|(e3&σ3&efs&?)];
+    rewrite ?eq_None_not_Some; auto.
+  { exfalso. eauto. }
+  destruct (elem_of_list_split t2 e2) as (t2'&t2''&->); auto.
+  right; exists (t2' ++ e3 :: t2'' ++ efs), σ3; econstructor; eauto.
+Qed.
+*)
+
+Section adequacy.
+Context {OpT: Type → Type}.
+Context `{Λ: Layer OpT}.
+Context `{irisG OpT Λ Σ}.
+(*
+Implicit Types e : expr Λ.
+*)
+Implicit Types P Q : iProp Σ.
+(*
+Implicit Types Φ : val Λ → iProp Σ.
+Implicit Types Φs : list (val Λ → iProp Σ).
+*)
+
+Notation world' E σ := (wsat ∗ ownE E ∗ state_interp σ)%I (only parsing).
+Notation world σ := (world' ⊤ σ) (only parsing).
+
+Notation wptp s t := ([∗ list] ef ∈ t, WP (projT2 ef) @ s; ⊤ {{ _, True }})%I.
+
+Lemma wp_step {T} s E e1 σ1 (e2: proc OpT T) σ2 efs Φ :
+  Λ.(exec_step) e1 σ1 σ2 (e2, efs) →
+  world' E σ1 ∗ WP e1 @ s; E {{ Φ }}
+  ==∗ ▷ |==> ◇ (world' E σ2 ∗ WP e2 @ s; E {{ Φ }} ∗ wptp s efs).
+Proof.
+  rewrite {1}wp_unfold /wp_pre. iIntros (?) "[(Hw & HE & Hσ) H]".
+  destruct (to_val e1) eqn:Hval.
+  { apply of_to_val in Hval. rewrite /of_val in Hval. subst.
+    destruct H as [Hσ Heq]. inversion Heq; subst.
+    iModIntro; rewrite wp_unfold //=. by iFrame.
+  }
+  rewrite // uPred_fupd_eq.
+  iMod ("H" $! σ1 with "Hσ [Hw HE]") as ">(Hw & HE & _ & H)"; first by iFrame.
+  iMod ("H" $! e2 σ2 efs with "[//] [$Hw $HE]") as ">(Hw & HE & H)".
+  iIntros "!> !>". by iMod ("H" with "[$Hw $HE]") as ">($ & $ & $)".
+Qed.
+
+Lemma wptp_step {T} s e1 t1 t2 σ1 σ2 Φ :
+  Λ.(exec_pool) ((existT T e1) :: t1) σ1 σ2 t2 →
+  world σ1 ∗ WP e1 @ s; ⊤ {{ Φ }} ∗ wptp s t1
+  ==∗ ∃ e2 t2', ⌜t2 = existT T e2 :: t2'⌝ ∗ ▷ |==> ◇ (world σ2 ∗ WP e2 @ s; ⊤ {{ Φ }} ∗ wptp s t2').
+Proof.
+  iIntros (Hstep%exec_pool_equiv_alt) "(HW & He & Ht)".
+  destruct Hstep as [T' e1' e2' efs [|? t1'] t2' Heq1 Heq2 Hstep]. rewrite //= in Heq1 Heq2.
+  - inversion Heq1 as [[Heq1' Heq2']]; subst.
+    assert (e1 = e1') by eauto with *; subst.
+    iExists e2', (t2' ++ efs); iSplitR; first eauto.
+    iFrame "Ht". iApply wp_step; eauto with iFrame.
+  - simplify_eq/=.
+    iExists e1, (t1' ++ existT _ e2' :: t2' ++ efs); iSplitR; first by eauto.
+    iDestruct "Ht" as "($ & He' & $)". iFrame "He".
+    iApply wp_step; eauto with iFrame.
+Qed.
+
+Lemma wptp_steps {T} s n e1 t1 t2 σ1 σ2 Φ :
+  bind_rep_n n (Λ.(exec_pool)) (existT T e1 :: t1) σ1 σ2 t2 →
+  world σ1 ∗ WP e1 @ s; ⊤ {{ Φ }} ∗ wptp s t1 ⊢
+  Nat.iter (S n) (λ P, |==> ▷ P) (∃ e2 t2',
+    ⌜t2 = existT T e2 :: t2'⌝ ∗ world σ2 ∗ WP e2 @ s; ⊤ {{ Φ }} ∗ wptp s t2').
+Proof.
+  revert e1 t1 t2 σ1 σ2; simpl; induction n as [|n IH]=> e1 t1 t2 σ1 σ2.
+  { inversion_clear 1; iIntros "(?&?&?)"; subst. iExists e1, t1; iFrame; auto. }
+  iIntros (Hsteps) "H". destruct Hsteps as (t1'&σ1'&Hexec&Hsteps).
+  iMod (wptp_step with "H") as (e1' t1'') "[% H]"; first eauto; simplify_eq.
+  iModIntro; iNext; iMod "H" as ">?". by iApply IH.
+Qed.
+
+Lemma bupd_iter_laterN_mono n P Q `{!Plain Q} :
+  (P ⊢ Q) → Nat.iter n (λ P, |==> ▷ P)%I P ⊢ ▷^n Q.
+Proof.
+  intros HPQ. induction n as [|n IH]=> //=. by rewrite IH bupd_plain.
+Qed.
+
+Lemma bupd_iter_frame_l n R Q :
+  R ∗ Nat.iter n (λ P, |==> ▷ P) Q ⊢ Nat.iter n (λ P, |==> ▷ P) (R ∗ Q).
+Proof.
+  induction n as [|n IH]; simpl; [done|].
+  by rewrite bupd_frame_l {1}(later_intro R) -later_sep IH.
+Qed.
+
+Lemma wptp_result {T T'} s n e1 t1 v2' t2 σ1 σ2 φ :
+  bind_rep_n n (Λ.(exec_pool)) (existT T e1 :: t1) σ1 σ2 (existT T' (of_val v2') :: t2) →
+  world σ1 ∗ WP e1 @ s; ⊤ {{ v, ∀ σ, state_interp σ ={⊤,∅}=∗ ⌜φ v σ⌝ }} ∗ wptp s t1
+  ⊢ ▷^(S (S n)) ⌜∃ v2, existT T (@of_val OpT _ v2) = existT T' (@of_val OpT _ v2') ∧ φ v2 σ2⌝.
+Proof.
+  intros. rewrite wptp_steps // laterN_later. apply: bupd_iter_laterN_mono.
+  iDestruct 1 as (e2 t2' ?) "((Hw & HE & Hσ) & H & _)"; simplify_eq.
+  assert (Ret v2' = e2) by eauto with *; subst.
+  iDestruct (wp_value_inv' with "H") as "H". rewrite uPred_fupd_eq.
+  iMod ("H" with "[$]") as ">(Hw & HE & H)".
+  iExists v2'. iMod ("H" with "Hσ [$]") as ">(_ & _ & %)"; auto.
+Qed.
+
+Lemma wp_safe {T} E (e: proc OpT T) σ Φ :
+  world' E σ -∗ WP e @ E {{ Φ }} ==∗ ▷ ⌜is_Some (to_val e) ∨ reducible e σ⌝.
+Proof.
+  rewrite wp_unfold /wp_pre. iIntros "(Hw&HE&Hσ) H".
+  destruct (to_val e) as [v|] eqn:?.
+  { iIntros "!> !> !%". left. by exists v. }
+  rewrite uPred_fupd_eq. iMod ("H" with "Hσ [-]") as ">(?&?&%&?)"; first by iFrame.
+  iIntros "!> !> !%". by right.
+Qed.
+
+Lemma wptp_safe {T T'} n (e1: proc OpT T) (e2: proc OpT T') t1 t2 σ1 σ2 Φ :
+  bind_rep_n n (Λ.(exec_pool)) (existT T e1 :: t1) σ1 σ2 t2 →
+  existT T' e2 ∈ t2 →
+  world σ1 ∗ WP e1 {{ Φ }} ∗ wptp NotStuck t1
+  ⊢ ▷^(S (S n)) ⌜is_Some (to_val e2) ∨ reducible e2 σ2⌝.
+Proof.
+  intros ? He2. rewrite wptp_steps // laterN_later. apply: bupd_iter_laterN_mono.
+  iDestruct 1 as (e2' t2' ?) "(Hw & H & Htp)"; simplify_eq.
+  apply elem_of_cons in He2 as [Heq|?].
+  - inversion Heq; subst.  assert (e2 = e2') as <- by eauto with *.
+    iMod (wp_safe with "Hw H") as "$".
+  - iMod (wp_safe with "Hw [Htp]") as "$".
+    iPoseProof (big_sepL_elem_of with "Htp") as "H"; eauto.
+Qed.
+
+Lemma wptp_invariance {T} s n e1 t1 t2 σ1 σ2 φ Φ :
+  bind_rep_n n (Λ.(exec_pool)) (existT T e1 :: t1) σ1 σ2 t2 →
+  (state_interp σ2 ={⊤,∅}=∗ ⌜φ⌝) ∗ world σ1 ∗ WP e1 @ s; ⊤ {{ Φ }} ∗ wptp s t1
+  ⊢ ▷^(S (S n)) ⌜φ⌝.
+Proof.
+  intros ?. rewrite wptp_steps // bupd_iter_frame_l laterN_later.
+  apply: bupd_iter_laterN_mono.
+  iIntros "[Hback H]"; iDestruct "H" as (e2' t2' ->) "[(Hw&HE&Hσ) _]".
+  rewrite uPred_fupd_eq.
+  iMod ("Hback" with "Hσ [$Hw $HE]") as "> (_ & _ & $)"; auto.
+Qed.
+End adequacy.
+
+(*
+Theorem wp_strong_adequacy {T} OpT Σ Λ `{invPreG Σ} s (e: proc OpT T) σ φ :
+  (∀ `{Hinv : invG Σ},
+     (|={⊤}=> ∃ stateI : State Λ → iProp Σ,
+       let _ : irisG OpT Λ Σ := IrisG _ _ _ Hinv stateI in
+       stateI σ ∗ WP e @ s; ⊤ {{ v, ∀ σ, stateI σ ={⊤,∅}=∗ ⌜φ v σ⌝ }})%I) →
+  adequate s e σ φ.
+Proof.
+  intros Hwp; split.
+  - intros σ' (T'&v') Hexec.
+    destruct Hexec as ([|(?&e')]&?&Hpartial&Hcheck).
+    { inversion Hcheck. }
+    destruct e'; inversion Hcheck; subst.
+    subst. destruct t'.
+    eapply (soundness (M:=iResUR Σ) _ (S (S n))).
+    iMod wsat_alloc as (Hinv) "[Hw HE]". specialize (Hwp _).
+    rewrite {1}uPred_fupd_eq in Hwp; iMod (Hwp with "[$Hw $HE]") as ">(Hw & HE & Hwp)".
+    iDestruct "Hwp" as (Istate) "[HI Hwp]".
+    iApply (@wptp_result _ _ (IrisG _ _ Hinv Istate)); eauto with iFrame.
+  - destruct s; last done. intros t2 σ2 e2 _ [n ?]%rtc_nsteps ?.
+    eapply (soundness (M:=iResUR Σ) _ (S (S n))).
+    iMod wsat_alloc as (Hinv) "[Hw HE]". specialize (Hwp _).
+    rewrite uPred_fupd_eq in Hwp; iMod (Hwp with "[$Hw $HE]") as ">(Hw & HE & Hwp)".
+    iDestruct "Hwp" as (Istate) "[HI Hwp]".
+    iApply (@wptp_safe _ _ (IrisG _ _ Hinv Istate)); eauto with iFrame.
+Qed.
+
+Theorem wp_adequacy Σ Λ `{invPreG Σ} s e σ φ :
+  (∀ `{Hinv : invG Σ},
+     (|={⊤}=> ∃ stateI : state Λ → iProp Σ,
+       let _ : irisG Λ Σ := IrisG _ _ Hinv stateI in
+       stateI σ ∗ WP e @ s; ⊤ {{ v, ⌜φ v⌝ }})%I) →
+  adequate s e σ (λ v _, φ v).
+Proof.
+  intros Hwp. apply (wp_strong_adequacy Σ _)=> Hinv.
+  iMod Hwp as (stateI) "[Hσ H]". iExists stateI. iIntros "{$Hσ} !>".
+  iApply (wp_wand with "H"). iIntros (v ? σ') "_".
+  iMod (fupd_intro_mask' ⊤ ∅) as "_"; auto.
+Qed.
+
+Theorem wp_invariance Σ Λ `{invPreG Σ} s e σ1 t2 σ2 φ :
+  (∀ `{Hinv : invG Σ},
+     (|={⊤}=> ∃ stateI : state Λ → iProp Σ,
+       let _ : irisG Λ Σ := IrisG _ _ Hinv stateI in
+       stateI σ1 ∗ WP e @ s; ⊤ {{ _, True }} ∗ (stateI σ2 ={⊤,∅}=∗ ⌜φ⌝))%I) →
+  rtc step ([e], σ1) (t2, σ2) →
+  φ.
+Proof.
+  intros Hwp [n ?]%rtc_nsteps.
+  eapply (soundness (M:=iResUR Σ) _ (S (S n))).
+  iMod wsat_alloc as (Hinv) "[Hw HE]". specialize (Hwp _).
+  rewrite {1}uPred_fupd_eq in Hwp; iMod (Hwp with "[$Hw $HE]") as ">(Hw & HE & Hwp)".
+  iDestruct "Hwp" as (Istate) "(HIstate & Hwp & Hclose)".
+  iApply (@wptp_invariance _ _ (IrisG _ _ Hinv Istate)); eauto with iFrame.
+Qed.
+
+(* An equivalent version that does not require finding [fupd_intro_mask'], but
+can be confusing to use. *)
+Corollary wp_invariance' Σ Λ `{invPreG Σ} s e σ1 t2 σ2 φ :
+  (∀ `{Hinv : invG Σ},
+     (|={⊤}=> ∃ stateI : state Λ → iProp Σ,
+       let _ : irisG Λ Σ := IrisG _ _ Hinv stateI in
+       stateI σ1 ∗ WP e @ s; ⊤ {{ _, True }} ∗ (stateI σ2 -∗ ∃ E, |={⊤,E}=> ⌜φ⌝))%I) →
+  rtc step ([e], σ1) (t2, σ2) →
+  φ.
+Proof.
+  intros Hwp. eapply wp_invariance; first done.
+  intros Hinv. iMod (Hwp Hinv) as (stateI) "(? & ? & Hφ)".
+  iModIntro. iExists stateI. iFrame. iIntros "Hσ".
+  iDestruct ("Hφ" with "Hσ") as (E) ">Hφ".
+  iMod (fupd_intro_mask') as "_"; last by iModIntro. solve_ndisj.
+Qed.
+*)
